Updates.

LC/NV/UTLC/Sub/SubIsDef.lean
@@ -8,15 +8,15 @@ set_option autoImplicit false
 open Term_
 
 
--- sub_is_def M x N means M [ x := N ] is defined
-inductive sub_is_def : Term_ → Symbol_ → Term_ → Prop
+-- sub_is_def_v3 M x N means M [ x := N ] is defined
+inductive sub_is_def_v3 : Term_ → Symbol_ → Term_ → Prop
 
 -- y [ x := N ] is defined
 | var
   (y : Symbol_)
   (x : Symbol_)
   (N : Term_) :
-  sub_is_def (var_ y) x N
+  sub_is_def_v3 (var_ y) x N
 
 -- P [ x := N ] is defined → Q [ x := N ] is defined → (P Q) [ x := N ] is defined
 | app
@@ -24,9 +24,9 @@ inductive sub_is_def : Term_ → Symbol_ → Term_ → Prop
   (Q : Term_)
   (x : Symbol_)
   (N : Term_) :
-  sub_is_def P x N →
-  sub_is_def Q x N →
-  sub_is_def (app_ P Q) x N
+  sub_is_def_v3 P x N →
+  sub_is_def_v3 Q x N →
+  sub_is_def_v3 (app_ P Q) x N
 
 -- x = y → ( λ y . P ) [ x := N ] is defined
 | abs_same
@@ -35,7 +35,7 @@ inductive sub_is_def : Term_ → Symbol_ → Term_ → Prop
   (x : Symbol_)
   (N : Term_) :
   x = y →
-  sub_is_def (abs_ y P) x N
+  sub_is_def_v3 (abs_ y P) x N
 
 | abs_diff_nel
   (y : Symbol_)
@@ -44,7 +44,7 @@ inductive sub_is_def : Term_ → Symbol_ → Term_ → Prop
   (N : Term_) :
   ¬ x = y →
   x ∉ P.free_var_set →
-  sub_is_def (abs_ y P) x N
+  sub_is_def_v3 (abs_ y P) x N
 
 | abs_diff
   (y : Symbol_)
@@ -53,8 +53,8 @@ inductive sub_is_def : Term_ → Symbol_ → Term_ → Prop
   (N : Term_) :
   ¬ x = y →
   y ∉ N.free_var_set →
-  sub_is_def P x N →
-  sub_is_def (abs_ y P) x N
+  sub_is_def_v3 P x N →
+  sub_is_def_v3 (abs_ y P) x N
 
 
 -------------------------------------------------------------------------------
@@ -66,11 +66,11 @@ lemma lemma_1_2_5_i_a
   (x : Symbol_)
   (N : Term_)
   (h1 : x ∉ M.free_var_set) :
-  sub_is_def M x N :=
+  sub_is_def_v3 M x N :=
   by
   induction M
   case var_ y =>
-    exact sub_is_def.var y x N
+    exact sub_is_def_v3.var y x N
 
   case app_ P Q ih_P ih_Q =>
     unfold Term_.free_var_set at h1
@@ -78,12 +78,12 @@ lemma lemma_1_2_5_i_a
     obtain ⟨h1_left, h1_right⟩ := h1
     specialize ih_P h1_left
     specialize ih_Q h1_right
-    exact sub_is_def.app P Q x N ih_P ih_Q
+    exact sub_is_def_v3.app P Q x N ih_P ih_Q
 
   case abs_ y P _ =>
     by_cases h_xy : x = y
-    · exact sub_is_def.abs_same y P x N h_xy
-    · apply sub_is_def.abs_diff_nel y P x N h_xy
+    · exact sub_is_def_v3.abs_same y P x N h_xy
+    · apply sub_is_def_v3.abs_diff_nel y P x N h_xy
       unfold free_var_set at h1
       simp at h1
       tauto
@@ -95,7 +95,7 @@ lemma lemma_1_2_5_ii_right
 (x : Symbol_)
 (N : Term_)
 (z : Symbol_)
-(h1 : sub_is_def M x N)
+(h1 : sub_is_def_v3 M x N)
 (h2 : z ∈ (replace_free x N M).free_var_set) :
 (z ∈ M.free_var_set ∧ x ≠ z) ∨ (z ∈ N.free_var_set ∧ x ∈ M.free_var_set) := sorry
 
@@ -106,7 +106,7 @@ lemma lemma_1_2_5_ii_left
 (x : Symbol_)
 (N : Term_)
 (z : Symbol_)
-(h1 : sub_is_def M x N)
+(h1 : sub_is_def_v3 M x N)
 (h2 : (z ∈ M.free_var_set ∧ x ≠ z) ∨ (z ∈ N.free_var_set ∧ x ∈ M.free_var_set)) :
 z ∈ (replace_free x N M).free_var_set := sorry
 
@@ -117,7 +117,7 @@ lemma lemma_1_2_5_ii
 {x : Symbol_}
 {N : Term_}
 {z : Symbol_}
-(H1 : sub_is_def M x N) :
+(H1 : sub_is_def_v3 M x N) :
 z ∈ (replace_free x N M).free_var_set ↔
   (z ∈ M.free_var_set ∧ x ≠ z) ∨ (z ∈ N.free_var_set ∧ x ∈ M.free_var_set) :=
 sorry
@@ -127,40 +127,40 @@ sorry
 lemma lemma_1_2_5_iii_a
 {M : Term_}
 {x : Symbol_} :
-sub_is_def M x (var_ x) := sorry
+sub_is_def_v3 M x (var_ x) := sorry
 
 
 -- [1]
 lemma lemma_1_2_6_a_left
 (M N L : Term_)
 (x y : Symbol_)
-(h1 : sub_is_def M x N)
-(h2 : sub_is_def N y L)
-(h3 : sub_is_def (replace_free x N M) y L)
+(h1 : sub_is_def_v3 M x N)
+(h2 : sub_is_def_v3 N y L)
+(h3 : sub_is_def_v3 (replace_free x N M) y L)
 (h4 : x ≠ y)
 (h5 : x ∉ L.free_var_set ∨ y ∉ M.free_var_set) :
-sub_is_def M y L := sorry
+sub_is_def_v3 M y L := sorry
 
 
 -- [1]
 lemma lemma_1_2_6_a_right
 (M N L : Term_)
 (x y : Symbol_)
-(h1 : sub_is_def M x N)
-(h2 : sub_is_def N y L)
-(h3 : sub_is_def (replace_free x N M) y L)
+(h1 : sub_is_def_v3 M x N)
+(h2 : sub_is_def_v3 N y L)
+(h3 : sub_is_def_v3 (replace_free x N M) y L)
 (h4 : x ≠ y)
 (h5 : x ∉ L.free_var_set ∨ y ∉ M.free_var_set) :
-sub_is_def (replace_free y L M) x (replace_free y L N) := sorry
+sub_is_def_v3 (replace_free y L M) x (replace_free y L N) := sorry
 
 
 -- [1]
 lemma lemma_1_2_6_b
 (M N L : Term_)
 (x y : Symbol_)
-(h1 : sub_is_def M x N)
-(h2 : sub_is_def N y L)
-(h3 : sub_is_def (replace_free x N M) y L)
+(h1 : sub_is_def_v3 M x N)
+(h2 : sub_is_def_v3 N y L)
+(h3 : sub_is_def_v3 (replace_free x N M) y L)
 (h4 : x ≠ y)
 (h5 : x ∉ L.free_var_set ∨ y ∉ M.free_var_set) :
 replace_free y L (replace_free x N M) =
